feat: ematch theorem activation for `grind` (#6475)
This PR adds support for activating relevant theorems for the (WIP)
`grind` tactic. We say a theorem is relevant to a `grind` goal if the
symbols occurring in its patterns also occur in the goal.

src/Lean/Meta/Tactic/Grind/EMatchTheorem.lean
@@ -25,7 +25,15 @@ inductive Origin where
   | other
   deriving Inhabited, Repr
 
-structure TheoremPattern where
+/-- A unique identifier corresponding to the origin. -/
+def Origin.key : Origin → Name
+  | .decl declName => declName
+  | .fvar fvarId   => fvarId.name
+  | .stx id _      => id
+  | .other         => `other
+
+/-- A theorem for heuristic instantiation based on E-matching. -/
+structure EMatchTheorem where
   proof       : Expr
   numParams   : Nat
   patterns    : List Expr
@@ -34,16 +42,21 @@ structure TheoremPattern where
   origin      : Origin
   deriving Inhabited
 
-abbrev TheoremPatterns := SMap Name (List TheoremPattern)
+/-- The key is a symbol from `EMatchTheorem.symbols`. -/
+abbrev EMatchTheorems := PHashMap Name (List EMatchTheorem)
 
-builtin_initialize theoremPatternsExt : SimpleScopedEnvExtension TheoremPattern TheoremPatterns ←
+def EMatchTheorems.insert (s : EMatchTheorems) (thm : EMatchTheorem) : EMatchTheorems := Id.run do
+  let .const declName :: syms := thm.symbols
+    | unreachable!
+  let thm := { thm with symbols := syms }
+  if let some thms := s.find? declName then
+    return PersistentHashMap.insert s declName (thm::thms)
+  else
+    return PersistentHashMap.insert s declName [thm]
+
+private builtin_initialize ematchTheoremsExt : SimpleScopedEnvExtension EMatchTheorem EMatchTheorems ←
   registerSimpleScopedEnvExtension {
-    addEntry := fun s t => Id.run do
-      let .const declName :: _ := t.symbols | unreachable!
-      if let some ts := s.find? declName then
-        s.insert declName (t::ts)
-      else
-        s.insert declName [t]
+    addEntry := EMatchTheorems.insert
     initial  := .empty
   }
 
@@ -282,19 +295,23 @@ private def ppParamsAt (proof : Expr) (numParms : Nat) (paramPos : List Nat) : M
         msg := msg ++ m!"{x} : {← inferType x}"
     addMessageContextFull msg
 
-def addTheoremPattern (declName : Name) (numParams : Nat) (patterns : List Expr) : MetaM Unit := do
+def addEMatchTheorem (declName : Name) (numParams : Nat) (patterns : List Expr) : MetaM Unit := do
   let .thmInfo info ← getConstInfo declName
     | throwError "`{declName}` is not a theorem, you cannot assign patterns to non-theorems for the `grind` tactic"
   let us := info.levelParams.map mkLevelParam
   let proof := mkConst declName us
   let (patterns, symbols, bvarFound) ← NormalizePattern.main patterns
+  assert! symbols.all fun s => s matches .const _
   trace[grind.pattern] "{declName}: {patterns.map ppPattern}"
   if let .missing pos ← checkCoverage proof numParams bvarFound then
      let pats : MessageData := m!"{patterns.map ppPattern}"
      throwError "invalid pattern(s) for `{declName}`{indentD pats}\nthe following theorem parameters cannot be instantiated:{indentD (← ppParamsAt proof numParams pos)}"
-  theoremPatternsExt.add {
+  ematchTheoremsExt.add {
      proof, patterns, numParams, symbols
      origin := .decl declName
   }
+
+def getEMatchTheorems : CoreM EMatchTheorems :=
+  return ematchTheoremsExt.getState (← getEnv)
 
 end Lean.Meta.Grind
